Testing/src/Lib.hs
@@ -1,7 +1,7 @@
 module Lib
     ( someFunc
     ) where
-import Test.QuickCheck (quickCheck);
+import Test.QuickCheck (quickCheck, verboseCheck);
 import qualified Option;
 import qualified Product_Type;
 import qualified List;
@@ -10,7 +10,7 @@ import qualified Arith;
 import qualified Blockchain(Hash, Block_ext, T, genBlock, tree0, hashComparea, hashCompare,
               valid_blocks, valid_chain, best_c, allBlocksAppend, allBlocksa,
               valid_t, block_eq, allBlocks, get_first, best_chain, extendTree,
-              blockpool_eq, blocktree_eq, valid_chain_weak, valid_t_weak)
+              blockpool_eq, blocktree_eq, valid_chain_weak, valid_t_weak,blockpool_eq_set)
 import Test.QuickCheck.Property
 import qualified Data.Set as Set
 prop_evenNumberPlusOneIsOdd :: Integer -> Property
@@ -20,10 +20,10 @@ prop_overlySpecific :: Integer -> Integer -> Property
 prop_overlySpecific x y = x == 0 ==> x * y == 0
  
 prop_tree :: Blockchain.T -> Blockchain.Block_ext ()-> Property
-prop_tree t b = (not (Blockchain.blocktree_eq (Blockchain.extendTree t b) t)) ==> (Blockchain.blockpool_eq (Blockchain.allBlocks (Blockchain.extendTree t b)) ((Blockchain.allBlocks t)++[b]))
+prop_tree t b = (not (Blockchain.blocktree_eq (Blockchain.extendTree t b) t)) ==> (Blockchain.blockpool_eq_set (Blockchain.allBlocks (Blockchain.extendTree t b)) ((Blockchain.allBlocks t)++[b]))
 
 prop_valid_chain :: Integer -> Blockchain.T -> Property
-prop_valid_chain s t = ( (Blockchain.valid_t t)) ==> Blockchain.valid_chain(Blockchain.best_chain s t) == True
+prop_valid_chain s t = ((Blockchain.valid_t t)) ==> Blockchain.valid_chain(Blockchain.best_chain s t) == True
 
 
 -- Lemma one extension adds one to the set of allblocks in the tree
@@ -32,7 +32,7 @@ prop_valid_chain s t = ( (Blockchain.valid_t t)) ==> Blockchain.valid_chain(Bloc
 -- assumes"s≥0∧valid_t t" shows "valid_chain_(best_chain s t)
 
 someFunc :: IO ()
-someFunc = quickCheck (prop_tree)
+someFunc = quickCheck (prop_tree);
 
-
-
+-- Node (Block_ext 1 1 (H 1 2) 1 ()) Leaf Leaf
+-- Block_ext 2 1 (H 1 1) 1 ()
