Testing/src/List.hs
@@ -1,6 +1,6 @@
 {-# LANGUAGE EmptyDataDecls, RankNTypes, ScopedTypeVariables #-}
 
-module List(find, hd) where {
+module List(find, member, hd) where {
 
 import Prelude ((==), (/=), (<), (<=), (>=), (>), (+), (-), (*), (/), (**),
   (>>=), (>>), (=<<), (&&), (||), (^), (^^), (.), ($), ($!), (++), (!!), Eq,
@@ -12,6 +12,10 @@ import qualified Prelude;
 find :: forall a. (a -> Bool) -> [a] -> Maybe a;
 find uu [] = Nothing;
 find p (x : xs) = (if p x then Just x else find p xs);
+
+member :: forall a. (Eq a) => [a] -> a -> Bool;
+member [] y = False;
+member (x : xs) y = x == y || member xs y;
 
 hd :: forall a. [a] -> a;
 hd (x21 : x22) = x21;
