Testing/src/Set.hs
@@ -1,0 +1,27 @@
+{-# LANGUAGE EmptyDataDecls, RankNTypes, ScopedTypeVariables #-}
+
+module Set(Set(..), equal_set) where {
+
+import Prelude ((==), (/=), (<), (<=), (>=), (>), (+), (-), (*), (/), (**),
+  (>>=), (>>), (=<<), (&&), (||), (^), (^^), (.), ($), ($!), (++), (!!), Eq,
+  error, id, return, not, fst, snd, map, filter, concat, concatMap, reverse,
+  zip, null, takeWhile, dropWhile, all, any, Integer, negate, abs, divMod,
+  String, Bool(True, False), Maybe(Nothing, Just));
+import qualified Prelude;
+import qualified List;
+
+data Set a = Set [a] | Coset [a];
+
+member :: forall a. (Eq a) => a -> Set a -> Bool;
+member x (Coset xs) = not (List.member xs x);
+member x (Set xs) = List.member xs x;
+
+less_eq_set :: forall a. (Eq a) => Set a -> Set a -> Bool;
+less_eq_set (Coset []) (Set []) = False;
+less_eq_set a (Coset ys) = all (\ y -> not (member y a)) ys;
+less_eq_set (Set xs) b = all (\ x -> member x b) xs;
+
+equal_set :: forall a. (Eq a) => Set a -> Set a -> Bool;
+equal_set a b = less_eq_set a b && less_eq_set b a;
+
+}
